%----- it's needs a,b,m-------------
\begin{sagesilent}
linear_congruence = LinearCongruenceEquation(a, b, m)
step_vector = linear_congruence.intermediate_steps()
a1 = step_vector[0]
b1 = step_vector[1]
m1 = step_vector[2]
inverse_a = step_vector[3]
result = step_vector[4]
\end{sagesilent}
%------------------------------------
Primero hallamos $d=({\sage{a}},{\sage{m}})=\sage{linear_congruence.d}$
\begin{align*}
	\sage{a}x &\equiv \sage{b} \mod{\sage{m}}\\
	\sage{a1}x &\equiv \sage{b1} \mod{\sage{m1}}\quad(\text{Por \ref{th:moduleChange}})\\
	(\sage{inverse_a}\cdot\sage{a1})x &\equiv \sage{inverse_a}(\sage{b1}) \mod{\sage{m1}}\quad(\text{Operando por el inverso de }\sage{a1})\\
	x &\equiv \sage{result} \mod{\sage{m1}}.
\end{align*}
As√≠ que la soluciones incongruentes son \sagestr{linear_congruence.show_solution()}.

%\textbf{Falta nombrar pasos}